feat(lang): add Yield structural lemmas
Add generic expression, assignment, sequence, branch, while, and fork structural proof doors for the Yield language, including the public while invariant lemma.

AI-Assisted-By: GPT-5.5

theories/Lang/Yield/Ticl.v
@@ -19,7 +19,9 @@
     APIs are erased. *)
 From Stdlib Require Import
   Fin
+  Morphisms
   Nat
+  Program.Equality
   Strings.String.
 
 From ExtLib Require Import
@@ -38,10 +40,95 @@ From TICL Require Export
 From TICL Require Import
   ICTree.Core
   ICTree.Equ
-  ICTree.Interp.Core.
+  ICTree.Eq.Bind
+  ICTree.Events.Writer
+  ICTree.Interp.Core
+  ICTree.Interp.State
+  ICTree.Logic.AX
+  ICTree.Logic.AF
+  ICTree.Logic.Bind
+  ICTree.Logic.CanStep
+  ICTree.Logic.Iter
+  ICTree.Logic.State
+  ICTree.SBisim
+  Logic.Core.
 
-Import ICtree ICTreeNotations.
+Import ICtree ICTreeNotations TiclNotations.
+Local Open Scope ticl_scope.
 Local Open Scope ictree_scope.
+
+Local Typeclasses Transparent equ.
+Lemma interp_equ_hetero
+    {E F : Type} `{Encode E} `{Encode F} {X}
+    (h : E ~> ictree F) :
+  forall (x y : ictree E X),
+    x ≅ y -> @equ F _ X X eq (interp h x) (interp h y).
+Proof.
+  change (forall x y : ictree E X,
+             @equ E _ X X eq x y ->
+             @equ F _ X X eq (interp h x) (interp h y)).
+  __coinduction_equ RR IH; intros * EQ1.
+  setoid_rewrite unfold_iter.
+  step in EQ1; inv EQ1.
+  - setoid_rewrite bind_ret_l; reflexivity.
+  - setoid_rewrite bind_bind; setoid_rewrite bind_ret_l.
+    upto_bind_equ.
+    constructor. intros.
+    apply IH. apply H3.
+  - setoid_rewrite bind_ret_l.
+    constructor.
+    apply IH. apply H3.
+  - setoid_rewrite bind_bind.
+    upto_bind_equ.
+    setoid_rewrite bind_ret_l.
+    constructor.
+    apply IH. apply H3.
+Qed.
+
+#[local] Instance interp_equ_hetero_proper
+    {E F : Type} `{Encode E} `{Encode F} {X}
+    (h : E ~> ictree F) :
+  Proper (equ eq ==> equ eq) (@interp E _ _ _ _ _ h X).
+Proof.
+  intros x y Hxy.
+  now apply interp_equ_hetero.
+Qed.
+
+Lemma interp_bind_hetero
+    {E F : Type} `{Encode E} `{Encode F} {A B}
+    (h : E ~> ictree F) (t : ictree E A) (k : A -> ictree E B) :
+  interp h (x <- t;; k x) ≅ (x <- interp h t;; interp h (k x)).
+Proof.
+  revert t.
+  __coinduction_equ RR IH; intros.
+  rewrite (ictree_eta t).
+  rewrite unfold_bind, unfold_interp.
+  destruct (observe t) eqn:Hobs; cbn.
+  - rewrite unfold_interp.
+    cbn.
+    rewrite bind_ret_l.
+    rewrite unfold_interp.
+    reflexivity.
+  - rewrite unfold_interp.
+    cbn.
+    rewrite bind_br.
+    setoid_rewrite bind_guard.
+    constructor; intro i.
+    step; econstructor; intros.
+    apply IH.
+  - rewrite (@unfold_interp _ _ _ _ _ h (Guard t0)).
+    cbn.
+    rewrite bind_guard.
+    constructor.
+    apply IH.
+  - rewrite unfold_interp.
+    cbn.
+    rewrite bind_bind.
+    upto_bind_equ.
+    rewrite bind_guard.
+    constructor.
+    apply IH.
+Qed.
 
 (** Expression denotation constructor unfold facts. *)
 Lemma denote_exp_yvar name :
@@ -144,6 +231,715 @@ Proof. reflexivity. Qed.
 Lemma denote_stmt_flow_yyield :
   denote_stmt_flow YYield = (yyield;; Ret Fallthrough).
 Proof. reflexivity. Qed.
+
+(** Erased source-structural facts for the state-only TICL tier. *)
+Local Ltac unfold_erased_expression :=
+  unfold instr_exp_erased, interp_thread, interp_yield, instr_stateE;
+  cbn;
+  setoid_rewrite unfold_interp;
+  cbn.
+
+Local Ltac unfold_erased_statement :=
+  unfold instr_stmt_erased, interp_scheduled_erased, interp_yield,
+    interp_spawn, scheduled_visible, instr_stateE;
+  cbn;
+  setoid_rewrite unfold_interp;
+  cbn.
+
+Local Ltac step_erased_state :=
+  rewrite interp_state_tau, sb_guard;
+  setoid_rewrite unfold_interp;
+  cbn.
+
+Local Ltac expose_erased_get_result ctx :=
+  rewrite interp_state_tau, sb_guard;
+  change (resum_ret (inr (inr StateE.Get)) (resum_ret StateE.Get ctx))
+    with ctx;
+  setoid_rewrite unfold_interp;
+  cbn;
+  rewrite interp_state_tau, sb_guard;
+  setoid_rewrite unfold_interp;
+  cbn.
+
+Local Ltac step_erased_state3 :=
+  step_erased_state; step_erased_state; step_erased_state.
+
+(** Flow-preserving erased statement instrumentation for structural facts whose
+    contracts must expose [Fallthrough] versus [HaltThread].  The public
+    [instr_stmt_erased] remains the scheduled unit-returning view. *)
+Definition instr_stmt_flow_erased
+    (s : YStmt) (ctx : Ctx) : ictreeW Ctx (YStmtFlow * Ctx) :=
+  instr_stateE (interp_thread (denote_stmt_flow s)) ctx.
+
+Lemma axr_yexp_ylit : forall n n' ctx ctx' w w',
+    n = n' ->
+    ctx = ctx' ->
+    w = w' ->
+    not_done w ->
+    <[ {instr_exp_erased (YLit n) ctx},
+       w |= AX done= {(n', ctx')} w' ]>.
+Proof.
+  intros; subst.
+  unfold_erased_expression.
+  rewrite interp_state_ret.
+  now apply axr_ret.
+Qed.
+
+Lemma axr_yexp_yvar_some : forall name value ctx ctx' w w',
+    lookup name ctx = Some value ->
+    ctx = ctx' ->
+    w = w' ->
+    not_done w ->
+    <[ {instr_exp_erased (YVar name) ctx},
+       w |= AX done= {(value, ctx')} w' ]>.
+Proof.
+  intros; subst.
+  unfold_erased_expression.
+  eapply anr_state_bind_r_eq.
+  - rewrite interp_state_get.
+    now apply axr_ret.
+  - cbn.
+    rewrite interp_state_tau, sb_guard.
+    change (resum_ret (inr (inr StateE.Get)) (resum_ret StateE.Get ctx'))
+      with ctx'.
+    setoid_rewrite subst_ret_l.
+    cbn.
+    setoid_rewrite unfold_interp.
+    cbn.
+    rewrite interp_state_tau, sb_guard.
+    setoid_rewrite subst_ret_l.
+    cbn.
+    setoid_rewrite unfold_interp.
+    cbn.
+    change (alist_find RelDec_string name ctx') with (lookup name ctx').
+    destruct (lookup name ctx') eqn:Hlookup; try congruence.
+    inv H.
+    cbn.
+    rewrite bind_ret_l.
+    repeat (rewrite interp_state_tau, sb_guard).
+    change (resum_ret (inl Yield) (resum_ret Yield tt)) with tt.
+    rewrite subst_ret_l.
+    cbn.
+    setoid_rewrite unfold_interp.
+    cbn.
+    rewrite interp_state_tau, sb_guard.
+    rewrite subst_ret_l.
+    cbn.
+    setoid_rewrite unfold_interp.
+    cbn.
+    rewrite interp_state_ret.
+    now apply axr_ret.
+Qed.
+
+Lemma axr_yexp_yplus : forall a b x y value ctx ctx' w w',
+    <[ {instr_exp_erased a ctx}, w |= AX done= {(x, ctx)} w ]> ->
+    <[ {instr_exp_erased b ctx}, w |= AX done= {(y, ctx)} w ]> ->
+    value = (x + y)%nat ->
+    ctx = ctx' ->
+    w = w' ->
+    not_done w ->
+    <[ {instr_exp_erased (YPlus a b) ctx},
+       w |= AX done= {(value, ctx')} w' ]>.
+Proof.
+  intros a b x y value ctx ctx' w w' Ha Hb Hvalue Hctx Hw Hnd.
+  subst.
+  unfold instr_exp_erased, interp_thread, interp_yield, instr_stateE in *.
+  cbn.
+  rewrite !interp_bind_hetero.
+  rewrite !interp_state_bind.
+  eapply anr_bind_r_eq.
+  - exact Ha.
+  - cbn.
+    rewrite !interp_bind_hetero.
+    rewrite !interp_state_bind.
+    eapply anr_bind_r_eq.
+    + exact Hb.
+    + cbn.
+      rewrite !unfold_interp.
+      cbn.
+      rewrite interp_state_ret.
+      apply axr_ret; auto.
+Qed.
+
+Lemma axr_yexp_yminus : forall a b x y value ctx ctx' w w',
+    <[ {instr_exp_erased a ctx}, w |= AX done= {(x, ctx)} w ]> ->
+    <[ {instr_exp_erased b ctx}, w |= AX done= {(y, ctx)} w ]> ->
+    value = (x - y)%nat ->
+    ctx = ctx' ->
+    w = w' ->
+    not_done w ->
+    <[ {instr_exp_erased (YMinus a b) ctx},
+       w |= AX done= {(value, ctx')} w' ]>.
+Proof.
+  intros a b x y value ctx ctx' w w' Ha Hb Hvalue Hctx Hw Hnd.
+  subst.
+  unfold instr_exp_erased, interp_thread, interp_yield, instr_stateE in *.
+  cbn.
+  rewrite !interp_bind_hetero.
+  rewrite !interp_state_bind.
+  eapply anr_bind_r_eq.
+  - exact Ha.
+  - cbn.
+    rewrite !interp_bind_hetero.
+    rewrite !interp_state_bind.
+    eapply anr_bind_r_eq.
+    + exact Hb.
+    + cbn.
+      rewrite !unfold_interp.
+      cbn.
+      rewrite interp_state_ret.
+      apply axr_ret; auto.
+Qed.
+
+Lemma axr_yexp_ymult : forall a b x y value ctx ctx' w w',
+    <[ {instr_exp_erased a ctx}, w |= AX done= {(x, ctx)} w ]> ->
+    <[ {instr_exp_erased b ctx}, w |= AX done= {(y, ctx)} w ]> ->
+    value = (x * y)%nat ->
+    ctx = ctx' ->
+    w = w' ->
+    not_done w ->
+    <[ {instr_exp_erased (YMult a b) ctx},
+       w |= AX done= {(value, ctx')} w' ]>.
+Proof.
+  intros a b x y value ctx ctx' w w' Ha Hb Hvalue Hctx Hw Hnd.
+  subst.
+  unfold instr_exp_erased, interp_thread, interp_yield, instr_stateE in *.
+  cbn.
+  rewrite !interp_bind_hetero.
+  rewrite !interp_state_bind.
+  eapply anr_bind_r_eq.
+  - exact Ha.
+  - cbn.
+    rewrite !interp_bind_hetero.
+    rewrite !interp_state_bind.
+    eapply anr_bind_r_eq.
+    + exact Hb.
+    + cbn.
+      rewrite !unfold_interp.
+      cbn.
+      rewrite interp_state_ret.
+      apply axr_ret; auto.
+Qed.
+
+Lemma axr_yexp_yplus_ylit_ylit : forall x y value ctx ctx' w w',
+    value = (x + y)%nat ->
+    ctx = ctx' ->
+    w = w' ->
+    not_done w ->
+    <[ {instr_exp_erased (YPlus (YLit x) (YLit y)) ctx},
+       w |= AX done= {(value, ctx')} w' ]>.
+Proof.
+  intros; subst.
+  unfold_erased_expression.
+  repeat rewrite subst_ret_l.
+  cbn.
+  rewrite interp_state_ret.
+  now apply axr_ret.
+Qed.
+
+Lemma axr_yexp_yminus_ylit_ylit : forall x y value ctx ctx' w w',
+    value = (x - y)%nat ->
+    ctx = ctx' ->
+    w = w' ->
+    not_done w ->
+    <[ {instr_exp_erased (YMinus (YLit x) (YLit y)) ctx},
+       w |= AX done= {(value, ctx')} w' ]>.
+Proof.
+  intros; subst.
+  unfold_erased_expression.
+  repeat rewrite subst_ret_l.
+  cbn.
+  rewrite interp_state_ret.
+  now apply axr_ret.
+Qed.
+
+Lemma axr_yexp_ymult_ylit_ylit : forall x y value ctx ctx' w w',
+    value = (x * y)%nat ->
+    ctx = ctx' ->
+    w = w' ->
+    not_done w ->
+    <[ {instr_exp_erased (YMult (YLit x) (YLit y)) ctx},
+       w |= AX done= {(value, ctx')} w' ]>.
+Proof.
+  intros; subst.
+  unfold_erased_expression.
+  repeat rewrite subst_ret_l.
+  cbn.
+  rewrite interp_state_ret.
+  now apply axr_ret.
+Qed.
+
+Lemma axr_ystmt_yskip_erased : forall ctx ctx' w w',
+    ctx = ctx' ->
+    w = w' ->
+    not_done w ->
+    <[ {instr_stmt_erased YSkip ctx},
+       w |= AX done= {(tt, ctx')} w' ]>.
+Proof.
+  intros; subst.
+  unfold_erased_statement.
+  step_erased_state.
+  rewrite interp_state_ret.
+  now apply axr_ret.
+Qed.
+
+Lemma axax_ystmt_yyield_erased : forall ctx ctx' w w',
+    ctx = ctx' ->
+    w = w' ->
+    not_done w ->
+    <[ {instr_stmt_erased YYield ctx},
+       w |= AX AX done= {(tt, ctx')} w' ]>.
+Proof.
+  intros; subst.
+  unfold_erased_statement.
+  step_erased_state.
+  rewrite bind_ret_l.
+  cbn.
+  step_erased_state.
+  step_erased_state.
+  apply anr_state_br; split.
+  - csplit; auto.
+  - intro i; dependent destruction i.
+    + step_erased_state3.
+      rewrite interp_state_ret.
+      apply axr_ret; auto.
+    + inversion i.
+Qed.
+
+Lemma aur_ystmt_yyield_erased : forall ctx ctx' w w' ψ,
+    ctx = ctx' ->
+    w = w' ->
+    not_done w ->
+    <[ {instr_stmt_erased YYield ctx},
+       w |= ψ AU AX AX done= {(tt, ctx')} w' ]>.
+Proof.
+  intros; subst.
+  cleft.
+  now apply axax_ystmt_yyield_erased.
+Qed.
+
+Local Definition yassign_after_value
+    (name : var) (value : nat) : ictree YEff YStmtFlow :=
+  ctx <- yget;; yput (add name value ctx);; Ret Fallthrough.
+
+Local Lemma aur_yassign_after_value : forall name value ctx w ψ R,
+    <( {log (add name value ctx)}, w |= ψ )> ->
+    R (Fallthrough, add name value ctx)
+      (Obs (Log (add name value ctx)) tt) ->
+    <[ {instr_stateE (interp_thread (yassign_after_value name value)) ctx},
+       w |= ψ AU AX done R ]>.
+Proof.
+  intros name value ctx w ψ R Hlog HR.
+  pose proof (ticll_not_done unit _ _ _ Hlog) as Hnd.
+  unfold yassign_after_value, interp_thread, interp_yield, instr_stateE.
+  cbn.
+  setoid_rewrite unfold_interp.
+  cbn.
+  eapply aur_state_bind_r_eq.
+  - apply aur_get; auto; split; reflexivity.
+  - cbn.
+    expose_erased_get_result ctx.
+    eapply aur_state_bind_r_eq.
+    + apply aur_put; auto; split; reflexivity.
+    + cbn.
+      step_erased_state.
+      step_erased_state.
+      rewrite interp_state_ret.
+      cleft.
+      apply axr_ret; auto.
+      constructor.
+Qed.
+
+Local Lemma aul_yassign_after_value : forall name value ctx w ψ φ,
+    <( {log (add name value ctx)}, w |= ψ )> ->
+    <( {Ret (Fallthrough, add name value ctx)},
+       {Obs (Log (add name value ctx)) tt} |= φ )> ->
+    <( {instr_stateE (interp_thread (yassign_after_value name value)) ctx},
+       w |= ψ AU φ )>.
+Proof.
+  intros name value ctx w ψ φ Hlog Hret.
+  pose proof (ticll_not_done unit _ _ _ Hlog) as Hnd.
+  unfold yassign_after_value, interp_thread, interp_yield, instr_stateE.
+  cbn.
+  setoid_rewrite unfold_interp.
+  cbn.
+  eapply aul_state_bind_r_eq.
+  - apply aur_get; auto; split; reflexivity.
+  - cbn.
+    expose_erased_get_result ctx.
+    eapply aul_state_bind_r_eq.
+    + apply aur_put; auto; split; reflexivity.
+    + cbn.
+      step_erased_state.
+      step_erased_state.
+      rewrite interp_state_ret.
+      cleft.
+      exact Hret.
+Qed.
+
+Lemma aur_ystmt_yassign : forall name expr value ctx w ψ R,
+    <[ {instr_exp_erased expr ctx}, w |= AX done= {(value, ctx)} w ]> ->
+    <( {log (add name value ctx)}, w |= ψ )> ->
+    R (Fallthrough, add name value ctx)
+      (Obs (Log (add name value ctx)) tt) ->
+    <[ {instr_stmt_flow_erased (YAssign name expr) ctx},
+       w |= ψ AU AX done R ]>.
+Proof.
+  intros name expr value ctx w ψ R Hexp Hlog HR.
+  unfold instr_stmt_flow_erased, instr_exp_erased, interp_thread,
+    interp_yield, instr_stateE in *.
+  cbn.
+  rewrite !interp_bind_hetero.
+  rewrite !interp_state_bind.
+  eapply aur_bind_r_eq.
+  - cleft.
+    exact Hexp.
+  - cbn.
+    change (interp_state h_stateW
+              (interp handle_yield
+                 (interp handle_thread
+                    (ctx <- yget;; yput (add name value ctx);;
+                     Ret Fallthrough))) ctx)
+      with (instr_stateE (interp_thread (yassign_after_value name value)) ctx).
+    now apply aur_yassign_after_value.
+Qed.
+
+Lemma aul_ystmt_yassign : forall name expr value ctx w ψ φ,
+    <[ {instr_exp_erased expr ctx}, w |= AX done= {(value, ctx)} w ]> ->
+    <( {log (add name value ctx)}, w |= ψ )> ->
+    <( {Ret (Fallthrough, add name value ctx)},
+       {Obs (Log (add name value ctx)) tt} |= φ )> ->
+    <( {instr_stmt_flow_erased (YAssign name expr) ctx}, w |= ψ AU φ )>.
+Proof.
+  intros name expr value ctx w ψ φ Hexp Hlog Hret.
+  unfold instr_stmt_flow_erased, instr_exp_erased, interp_thread,
+    interp_yield, instr_stateE in *.
+  cbn.
+  rewrite !interp_bind_hetero.
+  rewrite !interp_state_bind.
+  eapply aul_bind_r_eq.
+  - cleft.
+    exact Hexp.
+  - cbn.
+    change (interp_state h_stateW
+              (interp handle_yield
+                 (interp handle_thread
+                    (ctx <- yget;; yput (add name value ctx);;
+                     Ret Fallthrough))) ctx)
+      with (instr_stateE (interp_thread (yassign_after_value name value)) ctx).
+    now apply aul_yassign_after_value.
+Qed.
+
+Lemma anr_ystmt_yseq_fallthrough : forall a b ctx ctx' w w' φ ψ,
+    <[ {instr_stmt_flow_erased a ctx},
+       w |= φ AN done= {(Fallthrough, ctx')} w' ]> ->
+    <[ {instr_stmt_flow_erased b ctx'}, w' |= φ AN ψ ]> ->
+    <[ {instr_stmt_flow_erased (YSeq a b) ctx}, w |= φ AN ψ ]>.
+Proof.
+  intros a b ctx ctx' w w' φ ψ Ha Hb.
+  unfold instr_stmt_flow_erased, interp_thread, interp_yield, instr_stateE in *.
+  cbn.
+  rewrite !interp_bind_hetero.
+  rewrite !interp_state_bind.
+  eapply anr_bind_r_eq; eauto.
+Qed.
+
+Lemma aur_ystmt_yseq_fallthrough : forall a b ctx ctx' w w' φ ψ,
+    <[ {instr_stmt_flow_erased a ctx},
+       w |= φ AU AX done= {(Fallthrough, ctx')} w' ]> ->
+    <[ {instr_stmt_flow_erased b ctx'}, w' |= φ AU ψ ]> ->
+    <[ {instr_stmt_flow_erased (YSeq a b) ctx}, w |= φ AU ψ ]>.
+Proof.
+  intros a b ctx ctx' w w' φ ψ Ha Hb.
+  unfold instr_stmt_flow_erased, interp_thread, interp_yield, instr_stateE in *.
+  cbn.
+  rewrite !interp_bind_hetero.
+  rewrite !interp_state_bind.
+  eapply aur_bind_r_eq; eauto.
+Qed.
+
+Lemma aul_ystmt_yseq_fallthrough : forall a b ctx ctx' w w' φ ψ,
+    <[ {instr_stmt_flow_erased a ctx},
+       w |= φ AU AX done= {(Fallthrough, ctx')} w' ]> ->
+    <( {instr_stmt_flow_erased b ctx'}, w' |= φ AU ψ )> ->
+    <( {instr_stmt_flow_erased (YSeq a b) ctx}, w |= φ AU ψ )>.
+Proof.
+  intros a b ctx ctx' w w' φ ψ Ha Hb.
+  unfold instr_stmt_flow_erased, interp_thread, interp_yield, instr_stateE in *.
+  cbn.
+  rewrite !interp_bind_hetero.
+  rewrite !interp_state_bind.
+  eapply aul_bind_r_eq; eauto.
+Qed.
+
+Lemma yseq_halt_propagates : forall a b ctx ctx' w w' φ,
+    <[ {instr_stmt_flow_erased a ctx},
+       w |= φ AU AX done= {(HaltThread, ctx')} w' ]> ->
+    not_done w' ->
+    <[ {instr_stmt_flow_erased (YSeq a b) ctx},
+       w |= φ AU AX done= {(HaltThread, ctx')} w' ]>.
+Proof.
+  intros a b ctx ctx' w w' φ Ha Hnd.
+  unfold instr_stmt_flow_erased, interp_thread, interp_yield, instr_stateE in *.
+  cbn.
+  rewrite !interp_bind_hetero.
+  rewrite !interp_state_bind.
+  eapply aur_bind_r_eq.
+  - exact Ha.
+  - cbn.
+    rewrite !unfold_interp.
+    cbn.
+    apply aur_state_ret; auto; split; reflexivity.
+Qed.
+
+Lemma aul_ystmt_yif : forall test then_branch else_branch condition ctx w φ ψ,
+    <[ {instr_exp_erased test ctx}, w |= AX done= {(condition, ctx)} w ]> ->
+    (if YieldSyntax.is_true condition then
+       <( {instr_stmt_flow_erased then_branch ctx}, w |= φ AU ψ )>
+     else
+       <( {instr_stmt_flow_erased else_branch ctx}, w |= φ AU ψ )>) ->
+    <( {instr_stmt_flow_erased (YIf test then_branch else_branch) ctx},
+       w |= φ AU ψ )>.
+Proof.
+  intros test then_branch else_branch condition ctx w φ ψ Htest Hbranch.
+  unfold instr_stmt_flow_erased, instr_exp_erased, interp_thread,
+    interp_yield, instr_stateE in *.
+  cbn.
+  rewrite !interp_bind_hetero.
+  rewrite !interp_state_bind.
+  eapply aul_bind_r_eq.
+  - cleft; exact Htest.
+  - cbn.
+    destruct (YieldSyntax.is_true condition); exact Hbranch.
+Qed.
+
+Lemma aur_ystmt_yif : forall test then_branch else_branch condition ctx w φ ψ,
+    <[ {instr_exp_erased test ctx}, w |= AX done= {(condition, ctx)} w ]> ->
+    (if YieldSyntax.is_true condition then
+       <[ {instr_stmt_flow_erased then_branch ctx}, w |= φ AU ψ ]>
+     else
+       <[ {instr_stmt_flow_erased else_branch ctx}, w |= φ AU ψ ]>) ->
+    <[ {instr_stmt_flow_erased (YIf test then_branch else_branch) ctx},
+       w |= φ AU ψ ]>.
+Proof.
+  intros test then_branch else_branch condition ctx w φ ψ Htest Hbranch.
+  unfold instr_stmt_flow_erased, instr_exp_erased, interp_thread,
+    interp_yield, instr_stateE in *.
+  cbn.
+  rewrite !interp_bind_hetero.
+  rewrite !interp_state_bind.
+  eapply aur_bind_r_eq.
+  - cleft; exact Htest.
+  - cbn.
+    destruct (YieldSyntax.is_true condition); exact Hbranch.
+Qed.
+
+(** Raw source-flow while unrolling facts.  These expose [YStmtFlow]
+    directly, avoiding any claim that the scheduled erased unit layer can
+    distinguish loop fallthrough from child-thread halt. *)
+Definition ywhile_iteration (test : YExp) (body : YStmt) :
+    ictree YEff (unit + YStmtFlow) :=
+  condition_value <- denote_exp test;;
+  if YieldSyntax.is_true condition_value then
+    flow <- denote_stmt_flow body;;
+    match flow with
+    | Fallthrough => Ret (inl tt)
+    | HaltThread => Ret (inr HaltThread)
+    end
+  else
+    Ret (inr Fallthrough).
+
+Lemma aul_ystmt_ywhile_true : forall test body condition w w' φ ψ,
+    <[ {denote_exp test}, w |= φ AU AX done= condition w ]> ->
+    YieldSyntax.is_true condition = true ->
+    <[ {denote_stmt_flow body},
+       w |= φ AU AX done= Fallthrough w' ]> ->
+    not_done w' ->
+    <( {denote_stmt_flow (YWhile test body)}, w' |= φ AU ψ )> ->
+    <( {denote_stmt_flow (YWhile test body)}, w |= φ AU ψ )>.
+Proof.
+  intros test body condition w w' φ ψ Htest Htrue Hbody Hnd Hloop.
+  cbn.
+  eapply aul_iter_next with (R := fun (_ : unit) w0 => w0 = w').
+  - eapply aur_bind_r_eq.
+    + exact Htest.
+    + rewrite Htrue.
+      eapply aur_bind_r_eq.
+      * exact Hbody.
+      * cbn.
+        cleft.
+        apply axr_ret; auto.
+        exists tt; split; auto.
+  - intros [] w0 ->.
+    exact Hloop.
+Qed.
+
+Lemma aul_ystmt_ywhile_false : forall test body condition w φ ψ,
+    <[ {denote_exp test}, w |= φ AU AX done= condition w ]> ->
+    YieldSyntax.is_true condition = false ->
+    <( {Ret Fallthrough}, w |= ψ )> ->
+    <( {denote_stmt_flow (YWhile test body)}, w |= φ AU ψ )>.
+Proof.
+  intros test body condition w φ ψ Htest Hfalse Hret.
+  pose proof Htest as Htest_not_done.
+  apply aur_not_done in Htest_not_done.
+  cbn.
+  rewrite unfold_iter.
+  eapply aul_bind_r_eq.
+  - eapply aur_bind_r_eq.
+    + exact Htest.
+    + rewrite Hfalse.
+      cbn.
+      cleft.
+      apply axr_ret.
+      * exact Htest_not_done.
+      * split; reflexivity.
+  - cbn.
+    cleft.
+    exact Hret.
+Qed.
+
+Lemma aul_ystmt_ywhile_halt : forall test body condition w w' φ ψ,
+    <[ {denote_exp test}, w |= φ AU AX done= condition w ]> ->
+    YieldSyntax.is_true condition = true ->
+    <[ {denote_stmt_flow body},
+       w |= φ AU AX done= HaltThread w' ]> ->
+    not_done w' ->
+    <( {Ret HaltThread}, w' |= ψ )> ->
+    <( {denote_stmt_flow (YWhile test body)}, w |= φ AU ψ )>.
+Proof.
+  intros test body condition w w' φ ψ Htest Htrue Hbody Hnd Hret.
+  cbn.
+  rewrite unfold_iter.
+  eapply aul_bind_r_eq.
+  - eapply aur_bind_r_eq.
+    + exact Htest.
+    + rewrite Htrue.
+      eapply aur_bind_r_eq.
+      * exact Hbody.
+      * cbn.
+        cleft.
+        apply axr_ret; auto.
+  - cbn.
+    cleft.
+    exact Hret.
+Qed.
+
+Lemma aur_ystmt_ywhile_true : forall test body condition w w' φ ψ,
+    <[ {denote_exp test}, w |= φ AU AX done= condition w ]> ->
+    YieldSyntax.is_true condition = true ->
+    <[ {denote_stmt_flow body},
+       w |= φ AU AX done= Fallthrough w' ]> ->
+    not_done w' ->
+    <[ {denote_stmt_flow (YWhile test body)}, w' |= φ AU AX ψ ]> ->
+    <[ {denote_stmt_flow (YWhile test body)}, w |= φ AU AX ψ ]>.
+Proof.
+  intros test body condition w w' φ ψ Htest Htrue Hbody Hnd Hloop.
+  cbn.
+  eapply aur_iter_next with (R := fun (_ : unit) w0 => w0 = w').
+  - eapply aur_bind_r_eq.
+    + exact Htest.
+    + rewrite Htrue.
+      eapply aur_bind_r_eq.
+      * exact Hbody.
+      * cbn.
+        cleft.
+        apply axr_ret; auto.
+        exists tt; split; auto.
+  - intros [] w0 ->.
+    exact Hloop.
+Qed.
+
+Lemma aur_ystmt_ywhile_false : forall test body condition w φ ψ,
+    <[ {denote_exp test}, w |= φ AU AX done= condition w ]> ->
+    YieldSyntax.is_true condition = false ->
+    <[ {Ret Fallthrough}, w |= AX ψ ]> ->
+    <[ {denote_stmt_flow (YWhile test body)}, w |= φ AU AX ψ ]>.
+Proof.
+  intros test body condition w φ ψ Htest Hfalse Hret.
+  pose proof Htest as Htest_not_done.
+  apply aur_not_done in Htest_not_done.
+  cbn.
+  rewrite unfold_iter.
+  eapply aur_bind_r_eq.
+  - eapply aur_bind_r_eq.
+    + exact Htest.
+    + rewrite Hfalse.
+      cbn.
+      cleft.
+      apply axr_ret.
+      * exact Htest_not_done.
+      * split; reflexivity.
+  - cbn.
+    cleft.
+    exact Hret.
+Qed.
+
+Lemma ag_ystmt_ywhile : forall test body (R : World YEff -> Prop) w φ,
+    R w ->
+    (forall w,
+        R w ->
+        <( {denote_stmt_flow (YWhile test body)}, w |= φ )> /\
+        <[ {ywhile_iteration test body}, w |= AX (φ AU AX done
+             {fun lr w' => exists i' : unit, lr = inl i' /\ R w'}) ]>) ->
+    <( {denote_stmt_flow (YWhile test body)}, w |= AG φ )>.
+Proof.
+  intros test body R w φ HR Hstep.
+  cbn.
+  change (ICtree.iter (fun _ : unit => ywhile_iteration test body) tt)
+    with (denote_stmt_flow (YWhile test body)).
+  eapply ag_iter with (R := fun (_ : unit) w => R w); eauto.
+  intros [] w0 HR0.
+  specialize (Hstep w0 HR0) as [Hφ Hnext].
+  split.
+  - exact Hφ.
+  - cbn.
+    exact Hnext.
+Qed.
+
+Lemma aur_ystmt_yassign_ylit_erased : forall name n ctx w ψ R,
+    <( {log (add name n ctx)}, w |= ψ )> ->
+    R (tt, add name n ctx) (Obs (Log (add name n ctx)) tt) ->
+    <[ {instr_stmt_erased (YAssign name (YLit n)) ctx},
+       w |= ψ AU AX done R ]>.
+Proof.
+  intros name n ctx w ψ R Hlog HR.
+  pose proof (ticll_not_done unit _ _ _ Hlog) as Hnd.
+  unfold_erased_statement.
+  eapply aur_state_bind_r_eq.
+  - apply aur_get; auto; split; reflexivity.
+  - cbn.
+    expose_erased_get_result ctx.
+    eapply aur_state_bind_r_eq.
+    + apply aur_put.
+      * exact Hlog.
+      * split; reflexivity.
+    + cbn.
+      step_erased_state3.
+      apply aur_state_ret; auto with ticl.
+Qed.
+
+Lemma aul_ystmt_yassign_ylit_erased : forall name n ctx w ψ φ,
+    <( {log (add name n ctx)}, w |= ψ )> ->
+    <( {Ret (tt, add name n ctx)},
+       {Obs (Log (add name n ctx)) tt} |= φ )> ->
+    <( {instr_stmt_erased (YAssign name (YLit n)) ctx}, w |= ψ AU φ )>.
+Proof.
+  intros name n ctx w ψ φ Hlog Hret.
+  pose proof (ticll_not_done unit _ _ _ Hlog) as Hnd.
+  unfold_erased_statement.
+  eapply aul_state_bind_r_eq.
+  - apply aur_get; auto; split; reflexivity.
+  - cbn.
+    expose_erased_get_result ctx.
+    eapply aul_state_bind_r_eq.
+    + apply aur_put.
+      * exact Hlog.
+      * split; reflexivity.
+    + cbn.
+      step_erased_state3.
+      apply aul_state_ret; auto with ticl.
+Qed.
 
 (** Scheduler one-step/case regression facts. *)
 Section SchedulerFacts.
@@ -354,6 +1150,97 @@ Proof.
            (fun _ : unit => denote_stmt YSkip)).
   solve_visible_regression.
 Qed.
+
+Definition yfork_body_fork_continuation
+    (body : YStmt) (in_child : bool) : thread Mem :=
+  ICtree.subst'
+    (fun _ : YStmtFlow => Ret tt)
+    (observe
+       (ICtree.subst'
+          (fun branch : bool =>
+             if branch then
+               denote_stmt_flow body;; Ret HaltThread
+             else
+               Ret Fallthrough)
+          (RetF in_child))).
+
+Lemma scheduled_visible_yfork_body_one_step : forall body,
+  observe (scheduled_visible (YFork body)) =
+    VisF ((inr (inl Spawn)) : yieldE + (spawnE + Mem))
+      (fun _ =>
+         schedule 2
+           (cons_pool (yfork_body_fork_continuation body true)
+              (replace_pool
+                 (fun _ : Fin.t 1 => denote_stmt (YFork body))
+                 Fin.F1 (yfork_body_fork_continuation body false)))
+           (Some (Fin.FS Fin.F1))).
+Proof.
+  intro body.
+  unfold scheduled_visible.
+  apply (@schedule_focused_fork Mem _ 0
+           (fun _ : Fin.t 1 => denote_stmt (YFork body))
+           Fin.F1
+           (yfork_body_fork_continuation body)).
+  solve_visible_regression.
+Qed.
+
+Lemma yfork_child_halts_after_body body :
+  yfork_body_fork_continuation body true =
+    ICtree.subst' (fun _ : YStmtFlow => Ret tt)
+      (observe (denote_stmt_flow body;; Ret HaltThread)).
+Proof. reflexivity. Qed.
+
+Lemma yfork_parent_falls_through body :
+  observe (yfork_body_fork_continuation body false) = RetF tt.
+Proof. solve_visible_regression. Qed.
+
+Definition yseq_yfork_body_rest_fork_continuation
+    (body rest : YStmt) (in_child : bool) : thread Mem :=
+  ICtree.subst'
+    (fun _ : YStmtFlow => Ret tt)
+    (observe
+       (ICtree.subst'
+          (fun flow : YStmtFlow =>
+             match flow with
+             | Fallthrough => denote_stmt_flow rest
+             | HaltThread => Ret HaltThread
+             end)
+          (observe
+             (ICtree.subst'
+                (fun branch : bool =>
+                   if branch then
+                     denote_stmt_flow body;; Ret HaltThread
+                   else
+                     Ret Fallthrough)
+                (RetF in_child))))).
+
+Lemma scheduled_visible_yseq_yfork_body_rest_one_step : forall body rest,
+  observe (scheduled_visible (YSeq (YFork body) rest)) =
+    VisF ((inr (inl Spawn)) : yieldE + (spawnE + Mem))
+      (fun _ =>
+         schedule 2
+           (cons_pool
+              (yseq_yfork_body_rest_fork_continuation body rest true)
+              (replace_pool
+                 (fun _ : Fin.t 1 =>
+                    denote_stmt (YSeq (YFork body) rest))
+                 Fin.F1
+                 (yseq_yfork_body_rest_fork_continuation body rest false)))
+           (Some (Fin.FS Fin.F1))).
+Proof.
+  intros body rest.
+  unfold scheduled_visible.
+  apply (@schedule_focused_fork Mem _ 0
+           (fun _ : Fin.t 1 => denote_stmt (YSeq (YFork body) rest))
+           Fin.F1
+           (yseq_yfork_body_rest_fork_continuation body rest)).
+  solve_visible_regression.
+Qed.
+
+Lemma yseq_yfork_body_rest_parent_runs_rest body rest :
+  observe (yseq_yfork_body_rest_fork_continuation body rest false) =
+    observe (denote_stmt rest).
+Proof. solve_visible_regression. Qed.
 
 Definition yfork_yield_fork_continuation (in_child : bool) : thread Mem :=
   ICtree.subst'
